\documentclass[11pt,landscape]{article}

% https://blmoistawinde.github.io/ml_equations_latex/

\usepackage{amsmath,amssymb}

\usepackage{multicol}

\usepackage{titling}
\date{} % no date

% https://kb.mit.edu/confluence/pages/viewpage.action?pageId=3907057
\usepackage[margin=0.5in]{geometry}

% https://tex.stackexchange.com/questions/24561/setting-the-column-gap-in-a-twocolumn-or-multicol-document
\setlength{\columnsep}{3cm}

\setlength{\droptitle}{-5em}   % This is your set screw

\newcommand{\indep}{\perp \!\!\! \perp}

\title{Machine Learning Advanced Topics Group Formulas \vspace{-4em}}

\begin{document}
\maketitle

\begin{multicols}{2}

%\begin{multicols}{3}{
\begin{equation}
	p(x,y) = p(x)p(y) -  x \indep y
\end{equation}

% Product Rule (6.22) p184
\begin{equation}
	p(x,y) = p(y|x)p(x) - (6.22)
\end{equation}

\begin{equation}
	\hat{y} = \beta_0 + \beta_1 x_1 \cdots + \beta_m x_p
\end{equation}

\begin{equation}
	\boldsymbol{Y} = \boldsymbol{x}^T \boldsymbol{\beta}
\end{equation}

\begin{equation}
Cov[x,y] = \mathbb{E}[xy]-\mathbb{E}[x]\mathbb{E}[y]
\end{equation}

\begin{equation}
Corr[x,y] = \frac{Cov[x,y]}{\sqrt{\mathbb{V}[x] \mathbb{V}[y]}}
\end{equation}

% p185
\begin{equation}
	p(x|y) = \frac{p(y|x)p(x)}{p(y)} - (6.23)
\end{equation}


\begin{equation}
odds = \frac{p(X)}{1-p(X)}
\end{equation}

\begin{equation}
X\sim \mathcal{N}(\mu,\sigma^2)
\end{equation}

\begin{equation}
	f(x) = \frac{1}{\sigma\sqrt{2\pi}}\exp(-\frac{1}{2\sigma^2}(x-\mu)^2) %{1+e^{-x}}
\end{equation}


\begin{equation}
	X \sim U(0, 1)
\end{equation}

\begin{equation}
	X^TX
\end{equation}

\begin{equation}
	XX^T
\end{equation}

\begin{equation}
	A = P D P^{-1}
\end{equation}

\begin{equation}
	A = U\Sigma V^T
\end{equation}

% Negative entropy - Example 7.3 p237
\begin{equation}
	f(x) = x\,log_2\,x
\end{equation}

% Jensen's Inequality (7.30) p236
\begin{equation}
	f(\theta x + (1-\theta)y) = \theta f(x) + (1-\theta)f(y)
\end{equation}

\begin{equation}
	t = \frac{\bar{X} - \mu}{\frac{\hat{\sigma}}{\sqrt{n}}}
\end{equation}



%

\begin{equation}
	\phi(x) = \frac{1}{1+e^{-x}}
\end{equation}

% ISLR (4.2))
\begin{equation}
	p(x) = \frac{e^{\beta_0 + \beta_1 x_1 \cdots + \beta_m x_p}}{1+e^{\beta_0 + \beta_1 x_1 \cdots + \beta_m x_p}}
\end{equation}

\begin{equation}
BCE = -(y\,log(p)+(1-y)log(1-p))
\end{equation}

\end{multicols}{2}

\end{document}
